{
 "cells": [
  {
   "cell_type": "markdown",
   "metadata": {},
   "source": [
    "# CSCI 5454 - Assigment 2 \n",
    "\n",
    "__Your Name:__ Shipra Behera\n",
    "\n",
    "__ Collaborated With: __\n",
    "\n",
    "This assignment is to be completed and uploaded to  moodle as a python3 notebook. \n",
    "  * Submission deadlines are posted on moodle. \n",
    "  * The questions  provided  below will ask you to either write code or  write answers in the form of markdown.\n",
    "  * Markdown syntax guide is here: [click here](https://github.com/adam-p/markdown-here/wiki/Markdown-Cheatsheet)\n",
    "  * Using markdown you can typeset formulae using latex. This way you can write nice readable answers with formulae like thus:\n",
    "> The algorithm runs in time $\\Theta\\left(n^{2.1\\log_2(\\log_2( n \\log^*(n)))}\\right)$, \n",
    "wherein $\\log^*(n)$ is the inverse _Ackerman_ function.\n",
    "\n",
    "__Double click anywhere on this box to find out how your instructor typeset it. Press Shift+Enter to go back. __\n"
   ]
  },
  {
   "cell_type": "markdown",
   "metadata": {},
   "source": [
    "## Problem 1: Fixed Point in an Array (15 points)\n",
    "\n",
    "__(A, 5 points)__ A fixed point of an array $A$, if it exists, is an index $i$ such that $A[i] = i$.\n",
    "Given a _sorted_ array $A$ of _distinct_ integers, return the index of the fixed point if one exists, or otherwise, return `-1` to signal that no fixed point exists. Your algorithm must be as efficient as possible."
   ]
  },
  {
   "cell_type": "code",
   "execution_count": 60,
   "metadata": {},
   "outputs": [],
   "source": [
    "def find_fixed_point(a):\n",
    "    # YOUR SOLUTION HERE\n",
    "    left = 0\n",
    "    right = len(a) - 1\n",
    "    while (left <= right):\n",
    "        mid = int(left + (right-1)/2)\n",
    "        if a[mid] == mid:\n",
    "            return mid\n",
    "        elif a[mid] < mid:\n",
    "            left = mid + 1\n",
    "        else:\n",
    "            right = mid - 1\n",
    "    return -1       \n",
    "    # END"
   ]
  },
  {
   "cell_type": "code",
   "execution_count": 61,
   "metadata": {},
   "outputs": [
    {
     "name": "stdout",
     "output_type": "stream",
     "text": [
      "j1= 2\n",
      "j2 =  -1\n",
      "j3 =  3\n",
      "j4 =  0\n",
      " num tests  =  10000\n",
      " num passed =  10000\n"
     ]
    }
   ],
   "source": [
    "## TESTING CODE : DO NOT EDIT\n",
    "from random import sample\n",
    "def find_fixed_point_very_naive(a):\n",
    "    n = len(a)\n",
    "    for i in range(0, n):\n",
    "        if a[i] == i:\n",
    "            return i\n",
    "    return -1\n",
    "\n",
    "a1 = [-1, 0, 2, 3, 10, 12]\n",
    "j1 = find_fixed_point(a1)\n",
    "print('j1=', j1)\n",
    "assert a1[j1] == j1, 'Failed test a1'\n",
    "\n",
    "a2 = [-1, 0, 4, 8, 15, 32]\n",
    "j2 = find_fixed_point(a2)\n",
    "print('j2 = ', j2)\n",
    "assert j2 == -1, ' Failed test a2'\n",
    "\n",
    "a3 = [0, 1, 2, 3, 4, 5, 6, 7, 9]\n",
    "j3 = find_fixed_point(a3)\n",
    "print('j3 = ', j3)\n",
    "assert a3[j3] == j3, ' Failed test a3'\n",
    "\n",
    "\n",
    "a4 = [0]\n",
    "j4 = find_fixed_point(a4)\n",
    "print('j4 = ', j4)\n",
    "assert a4[j4] == j4, ' Failed test a4'\n",
    "\n",
    "\n",
    "def test_find_fixed_point_code(n_tests, test_size):\n",
    "    n_passed = 0\n",
    "    for i in range(0, n_tests):\n",
    "        a = sorted( sample( range(-test_size,  test_size ), test_size))\n",
    "        j = find_fixed_point(a)\n",
    "        k = find_fixed_point_very_naive(a)\n",
    "        if (j >= 0 and a[j] != j): \n",
    "            print(' Code failed for input: ', a, 'returned : ', j, ' (not a fixed point) expected:', k)\n",
    "        elif (j == -1 and k != -1):\n",
    "            print(' Code failed for input: ', a, 'returned : ', j, ' but expected fixed point:', k)\n",
    "        else:\n",
    "            n_passed = n_passed + 1\n",
    "            \n",
    "    return n_passed\n",
    "\n",
    "n_tests = 10000\n",
    "n_passed = test_find_fixed_point_code(n_tests, 20)\n",
    "print(' num tests  = ', n_tests)\n",
    "print(' num passed = ', n_passed)\n",
    "\n",
    "## END TESTS For find_fixed_point\n"
   ]
  },
  {
   "cell_type": "markdown",
   "metadata": {},
   "source": [
    "__(B, 2 points)__  What is the running time for the algorithm in (A)? Derive a recurrence and writing down its solution."
   ]
  },
  {
   "cell_type": "markdown",
   "metadata": {},
   "source": [
    "## Answer (Expected Length: 4 lines)\n",
    "\n",
    "The running time is $\\Theta(\\log(n))$. <br/>\n",
    "The time to search an element in an array of n elements would be n/2 plus one comparison(con\n",
    "The recurrence is $T(n) = T(\\frac{n}{2}) + \\Theta(1)$<br/>\n",
    "Using master theorem, $a = 1, b= 2,$ from $(\\Theta(n^0)), c = 0$<br/>\n",
    "$\\epsilon = \\log_2{1} = 0$, which is equal to $c$. Thus from case 2 of master theorem, <br/>\n",
    "$T(n) = \\Theta(n^0\\log(n)) = \\Theta(\\log(n))$"
   ]
  },
  {
   "cell_type": "markdown",
   "metadata": {},
   "source": [
    "__(C, 7 points)__ You are given a series of coordinates starting from  $(x_0, y_0), (x_1, y_1), \\ldots, (x_{n-1}, y_{n-1})$, such that $x_0 < x_1 < \\cdots < x_{n-1}$ and $y_0 < y_1 < \\cdots < y_{n-1}$. \n",
    "Furthermore, you are given that $x_0 < y_0$ and $x_{n-1} > y_{n-1}$. Imagine a \"curve\" formed by the straight line segments joining successive coordinates $(x_i, y_i)$ and $(x_{i+1}, y_{i+1})$. For convenience assume that $x_i \\not= y_i$ for all points.\n",
    "\n",
    "Write an efficient algorithm to find at least one point  where the curve intersects the line $x = y$ (first convince yourself that such a point must exist). \n",
    "  * Input: two lists `xValues`, `yValues` of equal size containing the x and y coordinates, respectively.\n",
    "    * The sizes of the lists are at least two or more.\n",
    "    * Both lists are sorted in ascending order.\n",
    "  * Output: Return the index $i$ such that the point of intersection with $x = y$ lies on the line segment joining\n",
    "$(x_i, y_i)$ with $(x_{i+1}, y_{i+1})$. \n",
    "    * Note that your algorithm, if correct, will always succeed in finding an intersection point.\n",
    "    \n",
    "Running time of your algorithm must be $\\Theta(\\log_2(n))$.\n"
   ]
  },
  {
   "cell_type": "code",
   "execution_count": 62,
   "metadata": {},
   "outputs": [],
   "source": [
    "def findPointOfIntersection(xValues, yValues): \n",
    "    left = 0\n",
    "    right = len(xValues) - 1\n",
    "    while (left <= right):\n",
    "        mid = int((left + right) / 2)\n",
    "        #mid = int(left + (right-1)/2)\n",
    "        if (xValues[mid] <= yValues[mid] and xValues[mid+1] >= yValues[mid+1]):\n",
    "            return mid \n",
    "        if (xValues[mid] < yValues[mid]):\n",
    "            left = mid + 1\n",
    "        elif (xValues[mid] > yValues[mid]):\n",
    "            right = mid\n",
    "    return -1"
   ]
  },
  {
   "cell_type": "code",
   "execution_count": 63,
   "metadata": {},
   "outputs": [
    {
     "name": "stdout",
     "output_type": "stream",
     "text": [
      "j1 =  3\n",
      "j2 =  8\n",
      "j3 =  3\n",
      "j4 =  0\n",
      "All 100 tests passed\n",
      "All 100 tests passed\n"
     ]
    },
    {
     "data": {
      "text/plain": [
       "True"
      ]
     },
     "execution_count": 63,
     "metadata": {},
     "output_type": "execute_result"
    }
   ],
   "source": [
    "## test code\n",
    "## test code: do not edit\n",
    "from random import randint, sample\n",
    "\n",
    "def checkIntersection(xValues, yValues, i):\n",
    "    if (i < 0 or i >= len(xValues)):\n",
    "        return False\n",
    "    if (xValues[i] < yValues[i] and xValues[i+1] > yValues[i+1]):\n",
    "        return True\n",
    "    return False\n",
    "\n",
    "def isOK(xValues, yValues):\n",
    "    n = len(xValues)\n",
    "    assert (len(yValues) == n)\n",
    "    if (xValues[0] >= yValues[0]):\n",
    "        return False\n",
    "    if (xValues[n-1] <= yValues[n-1]):\n",
    "        return False\n",
    "    for i in range(n):\n",
    "        if (xValues[i] == yValues[i]):\n",
    "            return False\n",
    "        if (i < n-1 and xValues[i+1] <= xValues[i]):\n",
    "            return False\n",
    "        if (i < n-1 and yValues[i+1] <= yValues[i]):\n",
    "            return False\n",
    "    return True\n",
    "\n",
    "\n",
    "\n",
    "xValues1 = [-4, -1, 2, 3, 5, 7, 9]\n",
    "yValues1 = [ 0, 2, 3, 3.5, 4, 5, 7]\n",
    "j1 = findPointOfIntersection(xValues1, yValues1)\n",
    "print('j1 = ', j1)\n",
    "assert checkIntersection(xValues1, yValues1, j1) \n",
    "\n",
    "xValues2 = [-5, -4, -3, -2, -1, 0, 5, 10, 15, 20, 25]\n",
    "yValues2 = [ 0,  2, 4,  8, 10, 12, 14, 16, 18, 19, 22]\n",
    "j2 = findPointOfIntersection(xValues2, yValues2)\n",
    "print('j2 = ', j2)\n",
    "assert checkIntersection(xValues2, yValues2, j2) \n",
    "\n",
    "\n",
    "\n",
    "xValues3 = [-2, -1, 0, 1, 2]\n",
    "yValues3 = [ 0, 0.5, 1, 1.5, 1.75]\n",
    "j3 = findPointOfIntersection(xValues3, yValues3)\n",
    "print('j3 = ', j3)\n",
    "assert checkIntersection(xValues3, yValues3, j3) \n",
    "\n",
    "\n",
    "\n",
    "xValues4 = [-2, 2]\n",
    "yValues4 = [ 0, 1 ]\n",
    "j4 = findPointOfIntersection(xValues4, yValues4)\n",
    "print('j4 = ', j4)\n",
    "assert checkIntersection(xValues4, yValues4, j4) \n",
    "\n",
    "\n",
    "\n",
    "\n",
    "def testPointOfIntersection(size, numTrials):\n",
    "    numActual = 0\n",
    "    for j in range(numTrials):\n",
    "        yValues = list(range(size))\n",
    "        k = randint(1,size-2)\n",
    "        xValues = []\n",
    "        for i in range(k):\n",
    "            xValues.append(yValues[i] - 2)\n",
    "        for i in range(k, size):\n",
    "            xValues.append(yValues[i] + 2)\n",
    "        #print(xValues, yValues)\n",
    "        if (isOK(xValues, yValues)):\n",
    "            j = findPointOfIntersection(xValues, yValues)\n",
    "            numActual = numActual + 1\n",
    "            if (not checkIntersection(xValues, yValues, j)): \n",
    "                print(\"--- FAILED TEST -- \")\n",
    "                print(\"xValues:\", xValues)\n",
    "                print(\"yValues:\", yValues)\n",
    "                print(\"Your code returned:\", j)\n",
    "                print(\"--- End Fail Report -- \")\n",
    "                return False\n",
    "    print(\"All %d tests passed\"%numActual)\n",
    "    return True\n",
    "\n",
    "testPointOfIntersection(50, 100)\n",
    "testPointOfIntersection(75, 100)\n",
    "# end Test Code"
   ]
  },
  {
   "cell_type": "markdown",
   "metadata": {},
   "source": [
    "## Problem 2: FFT problem (15 points)\n",
    "\n",
    "Consider a sequence of numbers $(a_0, \\ldots, a_{n-1})$ and let $(A_0, A_1, \\ldots, A_{n-1})$ be its\n",
    "discrete fourier transform: \n",
    "\n",
    "$$ A_j = \\sum_{k=0}^{n-1} a_k (\\omega_n^{jk})$$\n",
    "\n",
    "where $\\omega_n = e^{\\left( \\frac{2 \\pi i }{n} \\right)}$\n",
    "\n",
    "\n",
    "__(A, 7 points)__  Consider the Fourier transform of the circular permutation $(a_1, a_2, \\ldots, a_{n-1}, a_0)$. Let us denote it as $( \\hat{A}_0, \\ldots, \\hat{A}_{n-1})$. Find an expression for $\\hat{A}_j$ in terms of $A_j$. **Hint** Use the fact that $\\omega_n^n = 1$.\n",
    "\n",
    "__(B, 8 points)__ Generalize part (A) for the circular permutation $(a_{p}, \\ldots, a_{n-1}, a_0, \\ldots, a_{p-1})$. Use the fact that $\\omega_n^{n+j} = \\omega_n^j$."
   ]
  },
  {
   "cell_type": "markdown",
   "metadata": {},
   "source": [
    "### Answer (15 lines)\n",
    "\n",
    "__(A)__\n",
    "$ A_j = \\sum_{k=0}^{n-1} a_k (\\omega_n^{jk})$ <br/>\n",
    "Using the above Discrete Fourier Transform, for circular permutation $(a_1, a_2, \\ldots, a_{n-1}, a_0)$, <br/>\n",
    "we get,  $\\hat{A}_j = a_1\\omega_n^{j.0} + a_2\\omega_n^{j.1} + \\cdots + a_{n-1}\\omega_n^{j(n-2)} + a_0\\omega_n^{j(n-1)}$<br/>\n",
    "$$\\implies \\hat{A}_j = a_0\\omega_n^{j(n-1)} + a_1\\omega_n^{j.0} + a_2\\omega_n^{j.1} + \\cdots + a_{n-1}\\omega_n^{j(n-2)} $$ <br/><br/>\n",
    "DFT of sequence $(a_0, \\ldots, a_{n-1})$, <br/>\n",
    "$A_j = a_0\\omega_n^{j.0} + a_1\\omega_n^{j.1} + a_2\\omega_n^{j.2} + \\cdots + a_{n-1}\\omega_n^{j(n-1)} $ <br/><br/>\n",
    "Since $\\omega_n^n = 1$ and $\\omega_n^0 = 1$ and $(\\omega_n^{n})^{j} = 1$, we can write the first term, $a_0\\omega_n^{j.0}$ as $a_0\\omega_n^{jn}$ <br/><br/>\n",
    "$\\implies A_j = a_0\\omega_n^{jn} + a_1\\omega_n^{j.1} + a_2\\omega_n^{j.2} + \\cdots + a_{n-1}\\omega_n^{j(n-1)} $ <br/><br/>\n",
    "Taking out $\\omega_n^{j}$ from each term, we get<br/>\n",
    "$A_j = a_0\\omega_n^{j(n-1)}\\omega_n^j + a_1\\omega_n^{j.0}\\omega_n^j + a_2\\omega_n^{j.1}\\omega_n^j + \\cdots + a_{n-1}\\omega_n^{j(n-2)}\\omega_n^j $ <br/><br/>\n",
    "$\\implies A_j = \\omega_n^j(a_0\\omega_n^{j(n-1)} + a_1\\omega_n^{j.0} + a_2\\omega_n^{j.1} + \\cdots + a_{n-1}\\omega_n^{j(n-2)}) $ <br/><br/>\n",
    "$$\\implies \\frac{A_j}{\\omega_n^j} = a_0\\omega_n^{j(n-1)} + a_1\\omega_n^{j.0} + a_2\\omega_n^{j.1} + \\cdots + a_{n-1}\\omega_n^{j(n-2)} $$ <br/>\n",
    "The right side of this equation is equal to $\\hat{A}_j$ which we derived before.<br/>\n",
    "Hence, $$\\hat{A}_j = \\frac{A_j}{\\omega_n^j}$$\n",
    "\n",
    "__(B)__\n",
    "Using the above Discrete Fourier Transform, for circular permutation $(a_{p}, \\ldots, a_{n-1}, a_0, \\ldots, a_{p-1})$, <br/>\n",
    "we get,  $\\hat{A}_j = a_p\\omega_n^{j.0} + a_{p+1}\\omega_n^{j.1} + \\cdots + a_{n-2}\\omega_n^{j(n-2-p)} + a_{n-1}\\omega_n^{j(n-1-p)}+ \\cdots + a_0\\omega_n^{j(n-p)} + a_1\\omega_n^{j(n-p+1)} + \\cdots + a_{p-1}\\omega_n^{j(n-1)}$<br/><br/>\n",
    "$\\implies \\hat{A}_j = \\sum_{k=p}^{n-1} a_k (\\omega_n^{j(k-p)}) + \\sum_{k=0}^{p-1} a_k (\\omega_n^{j(n-p+k)})$ <br/><br/>\n",
    "$\\hat{A}_j = \\sum_{k=p}^{n-1} a_k (\\omega_n^{jk})(\\omega_n^{-jp}) + \\sum_{k=0}^{p-1} a_k (\\omega_n^{j(n+k)})(\\omega_n^{-jp})$ <br/><br/>\n",
    "$\\omega_n^{-jp}$ is a constant inside the summation, so we can take that out from both terms<br/>\n",
    "$\\hat{A}_j = (\\omega_n^{-jp}) (\\sum_{k=p}^{n-1} a_k (\\omega_n^{jk}) + \\sum_{k=0}^{p-1} a_k (\\omega_n^{j(n+k)}))$ <br/><br/>\n",
    "\n",
    "Since, $\\omega_n^n = 1, \\omega_n^{n+j} = \\omega_n^n\\omega_n^j = \\omega_n^j$, we can write $(\\omega_n^{n+k})^{j}$ as $\\omega_n^{jk}$<br/>\n",
    "$\\implies \\hat{A}_j = (\\omega_n^{-jp}) (\\sum_{k=p}^{n-1} a_k (\\omega_n^{jk}) + \\sum_{k=0}^{p-1} a_k (\\omega_n^{jk}))$ <br/><br/>\n",
    "$\\implies \\hat{A}_j = (\\omega_n^{-jp}) (\\sum_{k=0}^{n-1} a_k (\\omega_n^{jk}) $ <br/><br/>\n",
    "Hence, $$\\hat{A}_j = \\frac{A_j}{\\omega_n^{jp}}$$"
   ]
  },
  {
   "cell_type": "markdown",
   "metadata": {},
   "source": [
    "## Problem 3:  Sum to Target (15 points)\n",
    "\n",
    "We have sets $S_1, S_2$ and $S_3$ that are all subsets of $\\{0, \\ldots, n-1\\}$  for a number $n > 0$.\n",
    "Each set is given to you as an array of booleans. Eg., for $n= 5$ and $S_1 = \\{1, 2, 4\\}$, we have the \n",
    "array $[0, 1, 1, 0, 1]$ that denotes the set $S_1$.\n",
    "\n",
    "__(A, 7 points)__  Given a target number $T$, find the number of  triples $(i_1, i_2, i_3)$ such that $i_1 \\in S_1$, $i_2 \\in S_2$ and $i_3 \\in S_3$ such that $i_1 + i_2 + i_3 = T$. Your algorithm must operate in running time $O(n \\log(n))$.\n",
    "\n",
    "__(B, 8 points)__ Find the number of  triples $(i_1, i_2, i_3)$ such that $i_1 \\in S_1$, $i_2 \\in S_2$ and $i_3 \\in S_3$ such that $i_1 + i_2 - i_3 = 0$. Your algorithm must operate in running time $O(n \\log(n))$.\n",
    "\n",
    "\n",
    "**Hint** Each part will use the following template. \n",
    "(a) make up polynomials $p_1, p_2 $ and $p_3$ according to the given sets. \n",
    "(b) multiply them together.\n",
    "(c) read off the answer from the result."
   ]
  },
  {
   "cell_type": "markdown",
   "metadata": {},
   "source": [
    "### Answer (Expected: 10 lines)\n",
    "\n",
    "__(A)__ <br/>\n",
    "We can write each polynomial as $$p_i = \\sum_{j=0}^{length(S_i)} S_i[j]x^j$$ <br/>\n",
    "where $j=0$ to length$(S_i)$, and $S_i[j]$ is each element of the boolean array, and $i = 1, 2,3 $<br/>\n",
    "We can multiply polynomials, $\\prod_{i=1}^{3}p_i$, using FFT which will take $O(n \\log(n))$ running time. <br/>\n",
    "By looking at the coefficient of $x^T$ in the resulting polynomial, we will get the number of triplets such that $i_1 + i_2 + i_3 = T$, because it is the sum of all the right products.\n",
    "\n",
    "__(B)__ <br/>\n",
    "Adding $n$ on both sides of the equation, we get $i_1 + i_2 + (n - i_3) = n$ <br/>\n",
    "Thus, for $i = 1, 2$, we can write each polynomial as $$p_i = \\sum_{j=0}^{length(S_i)} S_i[j]x^j$$  <br/>\n",
    "and for $i = 3$, $$p_i = \\sum_{j=0}^{length(S_i)} S_i[j]x^{n-j}$$ <br/>\n",
    "where $j=0$ to length$(S_i)$, and $S_i[j]$ is each element of the boolean array.<br/>\n",
    "We can multiply polynomials, $\\prod_{i=1}^{3}p_i$, using FFT which will take $O(n \\log(n))$ running time. <br/>\n",
    "Since the target number is $n$, by looking at the coefficient of $x^n$ in the resulting polynomial, we will get the number of triplets such that $i_1 + i_2 + n - i_3 = n \\implies i_1 + i_2 - i_3 = 0$."
   ]
  },
  {
   "cell_type": "markdown",
   "metadata": {},
   "source": [
    "## Problem 4 (15 points)\n",
    "\n",
    "Show that the summation \n",
    "\n",
    "$$ \\sum_{j=0}^{n-1} \\left( \\sum_{k=0}^{n-1} a_k \\omega^{jk}\\right)  (\\overline{\\omega})^{j \\color{red}{m}} = n a_{\\color{red}{m}} $$\n",
    "for $m = 0, \\ldots, n-1$. Here $\\omega$ is the $n^{th}$ root of unity and $\\overline{\\omega} = \\omega^{-1}$.\n",
    "This establishes the fact that the inverse of the FFT is just the same algorithm using $\\overline{\\omega}$ instead of $\\omega$, as discussed in class.\n",
    "\n",
    "**Hints** Do not panic!!  \n",
    "\n",
    "1. Bring the $(\\overline{\\omega})^{j \\color{red}{m}}$ term into the summation, using the fact that $\\overline{\\omega} = \\omega^{-1}$.\n",
    "\n",
    "2. Next, change the order of summation taking each $a_k$ out in common.\n",
    "\n",
    "3. Use the geometric series summation and you will see all coefficients cancel to $0$ other than that for $a_m$.\n",
    "\n",
    "4. Arrive at the answer."
   ]
  },
  {
   "cell_type": "markdown",
   "metadata": {},
   "source": [
    "## Solution (Expected Length: 15 lines)\n",
    "\n",
    "\n",
    "$ \\sum_{j=0}^{n-1} \\left( \\sum_{k=0}^{n-1} a_k \\omega^{jk}\\right)  (\\overline{\\omega})^{j \\color{red}{m}}$<br/>\n",
    "\n",
    "$\\overline{\\omega} = \\omega^{-1}$\n",
    "$\\implies (\\overline{\\omega})^{j \\color{red}{m}} = ({\\omega})^{-j \\color{red}{m}}$<br/>\n",
    "Bringing this term into the summation, we get <br/>\n",
    "$ \\sum_{j=0}^{n-1} \\left( \\sum_{k=0}^{n-1} a_k \\omega^{jk}\\right)  ({\\omega})^{-j \\color{red}{m}} =  \\sum_{j=0}^{n-1} \\left( \\sum_{k=0}^{n-1} a_k \\omega^{jk} ({\\omega})^{-j \\color{red}{m}} \\right)$, because $({\\omega})^{-j \\color{red}{m}}$ is indepedent of k <br/>\n",
    "$ =  \\sum_{j=0}^{n-1} \\left( \\sum_{k=0}^{n-1} a_k \\omega^{jk-jm} \\right)$<br/>\n",
    "$ =  \\sum_{j=0}^{n-1} \\left( \\sum_{k=0}^{n-1} a_k \\omega^{j(k-m)} \\right)$<br/>\n",
    "Since this is a finite summation, we can change the order of summation <br/>\n",
    "$ =  \\sum_{k=0}^{n-1} \\left( \\sum_{j=0}^{n-1} a_k \\omega^{j(k-m)} \\right)$<br/>\n",
    "This makes $a_k$ a constant inside the second summation, so we can take that out as common <br/>\n",
    "$ =  \\sum_{k=0}^{n-1} a_k \\left( \\sum_{j=0}^{n-1} \\omega^{j(k-m)} \\right)$<br/>\n",
    "Now, lets consider 2 cases:\n",
    "1. $ k \\neq m$, let $ p = k-m $ <br/>\n",
    "$\\sum_{j=0}^{n-1} \\omega^{j(k-m)}  = \\omega^{0p} + \\omega^{1p} + \\omega^{2p} + \\cdots + \\omega^{(n-1)p}$,\n",
    "which is a geometric series with $\\omega^p$ as the common ratio. This summation gives <br/>\n",
    "$\\sum_{j=0}^{n-1} \\omega^{j(k-m)} = \\frac{1 - \\omega^{np}}{1 - \\omega^p}$ <br/>\n",
    "Since, $\\omega_n^n = 1 \\implies (\\omega_n^{np}) = (\\omega_n^{n})^{p} = 1$. Thus, $\\frac{1 - \\omega^{np}}{1 - \\omega^p} = 0$<br/>\n",
    "$ \\sum_{k=0}^{n-1} a_k \\left( \\sum_{j=0}^{n-1} \\omega^{j(k-m)} \\right) = 0$ <br/>\n",
    "\n",
    "2. $ k = m$ <br/>\n",
    "$ \\sum_{k=0}^{n-1} a_m \\left( \\sum_{j=0}^{n-1} \\omega^{j(k-m)} \\right) = \\sum_{k=0}^{n-1} a_m \\left( \\sum_{j=0}^{n-1} \\omega^{0} \\right) = \\sum_{k=0}^{n-1} a_m  = n a_{\\color{red}{m}} $ <br/>\n",
    "Hence proved."
   ]
  },
  {
   "cell_type": "code",
   "execution_count": null,
   "metadata": {},
   "outputs": [],
   "source": []
  }
 ],
 "metadata": {
  "kernelspec": {
   "display_name": "Python 3",
   "language": "python",
   "name": "python3"
  },
  "language_info": {
   "codemirror_mode": {
    "name": "ipython",
    "version": 3
   },
   "file_extension": ".py",
   "mimetype": "text/x-python",
   "name": "python",
   "nbconvert_exporter": "python",
   "pygments_lexer": "ipython3",
   "version": "3.5.5"
  }
 },
 "nbformat": 4,
 "nbformat_minor": 2
}
