{
 "cells": [
  {
   "cell_type": "markdown",
   "metadata": {},
   "source": [
    "# CSCI 5454 Assignment 3 \n",
    "\n",
    "Your Name Here: Shipra Behera "
   ]
  },
  {
   "cell_type": "markdown",
   "metadata": {},
   "source": [
    "## Problem 1: Axioms of Probability (20 points)\n",
    "\n",
    "Let $A$ be a sample space with a set of events $\\{ \\emptyset, E_1, \\ldots, E_n, A \\}$.  We covered the basic axioms\n",
    "of probability in class and recall a few of these axioms here.\n",
    "- $p(\\emptyset) = 0, p(A) = 1$.\n",
    "- $p(E_i) \\geq 0$ and $p(E_i) \\leq 1$ for all events $E_i$.\n",
    "- If $E_1, E_2, \\ldots, E_n$ are pairwise disjoint then $p(E_1 \\cup E_2 \\cup \\cdots \\cup E_n) = p(E_1) + \\cdots + p(E_n) $.\n",
    "\n",
    "Your proof can only use facts about sets, the  axioms above and previously proven facts in this problem. \n",
    "Please write down your proof as a bulleted list as shown below.\n",
    "\n",
    "> __Example__ Prove that if $E_1 \\subseteq E_2$ then $p(E_2 \\setminus E_1) = p(E_2) - p(E_1)$.\n",
    "\n",
    "> __Proof:__  \n",
    "> 1. $E_2 = E_1 \\cup  (E_2 \\setminus E_1) $.\n",
    "> 2. The sets $E_1, (E_2 \\setminus E_1) $ are disjoint. \n",
    "> 3. Therefore, $p(E_2) = p(E_1) + p(E_2 \\setminus E_1)$ (axiom).  \n",
    "> 4. Rearranging, $p(E_2 \\setminus E_1) = p(E_2) - p(E_1)$.\n",
    "\n",
    "(A) Prove that if $E_1 \\subseteq E_2$ then \n",
    "\n",
    "$$p(E_1) \\leq p(E_2)$$.\n",
    "\n",
    "(B) Prove the inclusion-exclusion principle: \n",
    "\n",
    "$$p(E_1 \\cup E_2) = p(E_1) + p(E_2) - p(E_1 \\cap E_2)\\,.$$\n",
    "\n",
    "(C) Prove Boole's Inequality:\n",
    "\n",
    "$$p(E_1) + p(E_2) - 1 \\leq p(E_1 \\cup E_2) \\leq p(E_1) + p(E_2)\\,.$$\n",
    "\n",
    "\n",
    "\n",
    "(D) Prove Frechet's Inequality:\n",
    "\n",
    "$$p(E_1) + p(E_2) -1 \\leq p(E_1 \\cap E_2) \\leq \\min( p(E_1), p(E_2) )\\,. $$\n",
    "\n",
    "\n"
   ]
  },
  {
   "cell_type": "markdown",
   "metadata": {},
   "source": [
    "## Solution (Expected Length: 25 lines)\n",
    "\n",
    "\n",
    "**(A)**<br/>\n",
    ">1.If $E_1 \\subseteq E_2$ then $E_2 = E_1 \\cup  (E_2 \\setminus E_1) $ <br/>\n",
    "\n",
    ">2.sets $E_1, (E_2 \\setminus E_1) $ are disjoint <br/>\n",
    "\n",
    ">3.Thus, from axiom, $p(E_2) = p(E_1) + p(E_2 \\setminus E_1)$ <br/>\n",
    "\n",
    ">4.By axiom of probability, $p(E_2 \\setminus E_1) \\geq 0$ <br/>\n",
    "\n",
    ">5.Hence, $p(E_2) \\geq p(E_1)$ or, $p(E_1) \\leq p(E_2)$<br/>\n",
    "\n",
    "**(B)**<br/>\n",
    "\n",
    ">1.$E_1 \\cup E_2$ can be written as $(E_1 \\setminus (E_1 \\cap E_2)) \\cup (E_2 \\setminus (E_1 \\cap E_2)) \\cup (E_1 \\cap E_2)$, where  $(E_1 \\setminus (E_1 \\cap E_2)), (E_2 \\setminus (E_1 \\cap E_2)), (E_1 \\cap E_2)$ are disjoint. <br/>\n",
    "\n",
    ">2.So by axiom of probability, $p(E_1 \\cup E_2) = p(E_1 \\setminus (E_1 \\cap E_2)) + p(E_2 \\setminus (E_1 \\cap E_2)) + p(E_1 \\cap E_2)$. <br/>\n",
    "\n",
    ">3.$(E_1 \\cap E_2) \\subseteq E_1$. Therefore from axiom, $p(E_1) = p(E_1 \\setminus (E_1 \\cap E_2)) + p(E_1 \\cap E_2)$, <br/>\n",
    "$\\implies p(E_1 \\setminus (E_1 \\cap E_2))  = p(E_1) - p(E_1 \\cap E_2)$ <br/>\n",
    "\n",
    ">4.Similarly, $p(E_2 \\setminus (E_1 \\cap E_2))  = p(E_2) - p(E_1 \\cap E_2)$.  <br/>\n",
    "\n",
    ">5.$\\implies p(E_1 \\cup E_2) = p(E_1) - p(E_1 \\cap E_2) + p(E_2) - p(E_1 \\cap E_2) + p(E_1 \\cap E_2) $. <br/>\n",
    "\n",
    ">6.$\\implies p(E_1 \\cup E_2) = p(E_1) + p(E_2) - p(E_1 \\cap E_2)$\n",
    "\n",
    "\n",
    "**(C)**<br/>\n",
    ">1.From B, $p(E_1 \\cup E_2) = p(E_1) + p(E_2) - p(E_1 \\cap E_2)$<br/>\n",
    "\n",
    ">2.By axiom of probability, $p(E_1 \\cap E_2)$ can take a minimum value of 0 and a maximum value of 1 <br/>\n",
    "\n",
    ">3.If it is 0, then $p(E_1 \\cup E_2) \\leq  p(E_1) + p(E_2)$ <br/>\n",
    "\n",
    ">4.If it is 1, then $p(E_1 \\cup E_2) \\geq  p(E_1) + p(E_2) - 1$ <br/>\n",
    "\n",
    ">5.Hence, $p(E_1) + p(E_2) - 1 \\leq p(E_1 \\cup E_2) \\leq p(E_1) + p(E_2)\\$ <br/>\n",
    "\n",
    "**(D)**<br/>\n",
    ">1.$p(E_1 \\cup E_2) = p(E_1) + p(E_2) - p(E_1 \\cap E_2)$<br/>\n",
    "\n",
    ">2.$p(E_1 \\cap E_2) = p(E_1) + p(E_2) - p(E_1 \\cup E_2)$<br/>\n",
    "\n",
    ">3.By axiom of probability, $p(E_1 \\cup E_2)$ can take a minimum value of 0 and a maximum value of 1 <br/>\n",
    "\n",
    ">4.If it is 1, then $p(E_1 \\cap E_2) \\geq  p(E_1) + p(E_2) - 1$ <br/>\n",
    "\n",
    ">5.If it is 0, then $p(E_1 \\cap E_2) = p(E_1) + p(E_2)$<br/>\n",
    "\n",
    ">6.We know that, $p(E_1 \\cap E_2) \\subseteq E_1$, and $p(E_1 \\cap E_2) \\subseteq E_2$ <br/>\n",
    "\n",
    ">7.From part(A), $p(E_1 \\cap E_2) \\leq E_1$, and $p(E_1 \\cap E_2) \\leq E_2$ <br/>\n",
    "\n",
    ">8.Thus combining the two, $p(E_1 \\cap E_2) \\leq \\min( p(E_1), p(E_2)$ <br/>\n",
    "\n",
    ">9.Hence, $p(E_1) + p(E_2) -1 \\leq p(E_1 \\cap E_2) \\leq \\min( p(E_1), p(E_2) )$"
   ]
  },
  {
   "cell_type": "markdown",
   "metadata": {},
   "source": [
    "## Problem 2 (10 points)\n",
    "\n",
    "Let $X$ be a random variable that takes values in the range $\\{ 0, \\ldots, n \\} $. Show that \n",
    "\n",
    "$$ \\mathbb{E}(X) = \\sum_{i=1}^n \\mathbb{P}( X \\geq i ) = \\mathbb{P}( X \\geq 1 ) +  \\mathbb{P}( X \\geq 2  ) + \\cdots + \\mathbb{P}(X \\geq n) $$.\n",
    "\n",
    "__Hint:__ Note that $\\mathbb{E}(X) = 1 \\mathbb{P}(X = 1) + 2 \\mathbb{P}( X = 2) + \\cdots + n \\mathbb{P}(X = n)$. Show that the RHS of the equality is exactly this."
   ]
  },
  {
   "cell_type": "markdown",
   "metadata": {},
   "source": [
    "## Answer (Expected length: 6 lines)\n",
    "\n",
    "$\\mathbb{E}(X) = 0 \\mathbb{P}(X = 0) + 1 \\mathbb{P}(X = 1) + 2 \\mathbb{P}( X = 2) + \\cdots + n \\mathbb{P}(X = n)$<br/>\n",
    "\n",
    "Since X can take discrete values from $\\{ 0, \\ldots, n \\} $, $\\mathbb{P}(X = i)$ can be written as $[\\mathbb{P}(X \\geq{i}) - \\mathbb{P}(X \\geq(i+1)]$<br/>\n",
    "\n",
    "So, $\\mathbb{E}(X) =  1 [\\mathbb{P}(X \\geq1) - \\mathbb{P}(X \\geq2)] + 2 [\\mathbb{P}(X \\geq2) - \\mathbb{P}(X \\geq3)] + \\cdots + (n-1)[\\mathbb{P}(X \\geq{n-1}) - \\mathbb{P}(X \\geq{n})] + n[\\mathbb{P}(X \\geq{n}) - \\mathbb{P}(X \\geq{n+1})]$<br/>\n",
    "\n",
    "Since $X$ can only take values till n, the last term is $\\mathbb{P}(X \\geq{n+1}) = 0$ <br/>\n",
    "\n",
    "$\\implies \\mathbb{E}(X) =  \\mathbb{P}(X \\geq1) - \\mathbb{P}(X \\geq2) + 2\\mathbb{P}(X \\geq2) - 2\\mathbb{P}(X \\geq3) + \\cdots + (n-1)\\mathbb{P}(X \\geq{n-1}) - (n-1)\\mathbb{P}(X \\geq{n}) + n\\mathbb{P}(X \\geq{n})$ <br/>\n",
    "\n",
    "After cancelling out terms, we get  $\\mathbb{E}(X) = \\sum_{i=1}^n \\mathbb{P}( X \\geq i ) = \\mathbb{P}( X \\geq 1 ) +  \\mathbb{P}( X \\geq 2  ) + \\cdots + \\mathbb{P}(X \\geq n) $\n"
   ]
  },
  {
   "cell_type": "markdown",
   "metadata": {},
   "source": [
    "## Problem 3 (15 points)\n",
    "\n",
    "We draw two numbers independently and uniformly at random  from the set $\\{1, \\ldots, n\\}$ with replacement (i.e, the same number can be drawn twice). What is the expected value of the minimum of these two numbers? Show that this number is  $\\frac{n}{3} + O(1) $.\n",
    "\n",
    "\n",
    "\n",
    "__Hint:__ First calculate the probability that the smaller of the two numbers is $\\geq j$ for each $j \\in \\{ 1, \\ldots, n\\}$. Next use the result from the previous problem. Also note that $1^2 + 2^2 + \\cdots + n^2 = \\frac{n(n+1)(2n+1)}{6}$.\n",
    "\n",
    "__(B)__ Repeat the same calculation for the maximum of the two numbers.\n",
    "\n"
   ]
  },
  {
   "cell_type": "markdown",
   "metadata": {},
   "source": [
    "### Answer (Expected Length: 6 lines).\n",
    "In problem 2, we proved that $ \\mathbb{E}(X) = \\sum_{i=1}^n \\mathbb{P}( X \\geq i )$ <br/>\n",
    "\n",
    "Replacing $X$ with $\\min(X_1, X_2)$, we see that $ \\mathbb{E}(\\min(X_1, X_2)) = \\sum_{i=1}^n \\mathbb{P}( \\min(X_1, X_2) \\geq i )$ <br/>\n",
    "\n",
    "For the minimum of $X_1$ and $X_2$ to be $\\geq j$, where $j \\in \\{ 1, \\ldots, n\\}$, **both** $X_1$ and $X_2$ have to be $\\geq j$ <br/>\n",
    "\n",
    "We can write that $ \\mathbb{E}(\\min(X_1, X_2)) = \\sum_{j=1}^n \\mathbb{P}(X_1\\geq j)  \\mathbb{P}(X_2\\geq j)$ <br/>\n",
    "\n",
    "For any $X$, note that we can get $(X\\geq j)$ numbers in $n-(j-1)$ ways. Hence, the probability of getting $(X\\geq j)$ numbers is $\\frac{n-(j-1)}{n}$, $n$ being the total numbers. <br/>\n",
    "\n",
    "$$\\implies \\mathbb{E}(\\min(X_1, X_2)) = \\sum_{j=1}^n (\\frac{n-j+1}{n})^2 = \\frac{1}{n^2}\\sum_{j=1}^n (n-j+1)^2  = \\frac{1}{n^2}[n^2 + (n-1)^2 + \\cdots + 2^2 + 1^2]$$<br/>\n",
    "$$\\implies \\mathbb{E}(\\min(X_1, X_2)) = \\frac{1}{n^2}\\frac{n(n+1)(2n+1)}{6} = \\frac{2n^{2}+3n+1}{6n} = \\frac{n}{3}+ \\frac{1}{2} + \\frac{1}{6n} = \\frac{n}{3} + O(1)$$<br/>\n",
    "\n",
    "__(B)__<br/>\n",
    "Using the same derivation, $ \\mathbb{E}(\\max(X_1, X_2)) = \\sum_{j=1}^n \\mathbb{P}( \\max(X_1, X_2) \\geq j )$ <br/>\n",
    "For the maximum of $X_1$ and $X_2$ to be $\\geq j$, where $j \\in \\{ 1, \\ldots, n\\}$, **any one** of $X_1$ and $X_2$ has to be $\\geq j$ <br/>\n",
    "Probability that one of $X_1, X_2$ is $\\geq j$ is same as ($1 - \\mathbb{P}(X_1,X_2)<j$), i.e both are less than $j$ <br/>\n",
    "$$ \\mathbb{E}(\\max(X_1, X_2)) = \\sum_{j=1}^n 1 - (\\mathbb{P}(X_1,X_2)<j) = \\sum_{j=1}^n [1 - \\mathbb{P}(X_1<j)\\mathbb{P}(X_2<j) ]$$\n",
    "$$ \\implies \\mathbb{E}(\\max(X_1, X_2)) = \\sum_{j=1}^n [1 - (1-\\mathbb{P}(X_1\\geq j))(1-\\mathbb{P}(X_2\\geq j))]$$\n",
    "$$ \\implies \\mathbb{E}(\\max(X_1, X_2)) = \\sum_{j=1}^n [1 - (1-(\\frac{n-j+1}{n}))^2] \\implies \\mathbb{E}(\\max(X_1, X_2)) = \\sum_{j=1}^n [1 - (1+(\\frac{n-j+1}{n})^2 -2(\\frac{n-j+1}{n}))]$$\n",
    "$$ \\implies \\mathbb{E}(\\max(X_1, X_2)) = \\sum_{j=1}^n [ 2(\\frac{n-j+1}{n}) - (\\frac{n-j+1}{n})^2 ] \\implies \\mathbb{E}(\\max(X_1, X_2)) = \\frac{1}{n^2}\\sum_{j=1}^n [ n^2 - j^2 + 2j + 1 ]$$\n",
    "$$ \\implies \\mathbb{E}(\\max(X_1, X_2)) = \\frac{1}{n^2}\\frac{n(4n^2 + 3n - 1)}{6} \\implies \\mathbb{E}(\\max(X_1, X_2)) = \\frac{2n}{3}+ \\frac{1}{2} - \\frac{1}{6n} = \\frac{2n}{3} + O(1)$$"
   ]
  },
  {
   "cell_type": "markdown",
   "metadata": {},
   "source": [
    "## Problem 4  (10 points)\n",
    "\n",
    "\n",
    "Alice and Bob play the following game by tossing a fair (unbiased) coin. Each player takes turns starting with Alice's turn.\n",
    "- If Alice turns up heads she wins at once, or else Bob gets a turn.\n",
    "- If Bob turns up tails, he wins at once, or else Alice gets a turn.\n",
    "\n",
    "What is the probability that Alice wins?  What is the expected number of  tosses in the game?\n",
    "\n",
    "__(B, extra credit)__ Design a game between Alice and Bob where the probability that Bob wins is precisely $\\frac{21}{64}$. In each move of the game, you must specify which player gets a turn and what happens if that player wins a heads or a tails.\n",
    "\n"
   ]
  },
  {
   "cell_type": "markdown",
   "metadata": {},
   "source": [
    "### Answer (Expected Length: 4 lines).\n",
    "\n",
    "For ease of understanding and generalizing the problem, let us assume that probability that Alice throws head be $a_h$, Alice throws head be $a_t$, Bob throws head be $b_h$, and Bob throws tail be $b_t$, where Alice would win if $a_h$ comes up.\n",
    "Thus, we can see probability that Alice wins turns out to be like this:<br/>\n",
    "\n",
    "P(Alice wins) = $a_h$(when she wins on 1st toss) + $a_tb_ha_h$ (when she wins on 3rd toss) + $a_tb_ha_tb_ha_h$ (when she wins on 5th toss) + $\\cdots$ (and so on) <br/>\n",
    "\n",
    "This is a geometric series whose sum would be $\\frac{a_h}{1-a_tb_h}$<br/>\n",
    "Since it is a fair coin, we can replace those probablities by $\\frac{1}{2}$. Hence **P(Alice wins) = $\\frac{2}{3}$**\n",
    "\n",
    "The coin would be tossed until either Alice or Bob wins, i.e keep tossing until Alice throws a head or Bob throws a tail. Using the naming convention as above, and assuming $X$ is the number of tosses, we can write that<br/>\n",
    "$\\mathbb{E}(X) = 1 \\mathbb{P}(X = 1) + 2 \\mathbb{P}( X = 2) + \\cdots $<br/>\n",
    "i.e game ends after 1 toss, game ends after 2nd toss, and so on... <br/>\n",
    "$\\implies \\mathbb{E}(X) = a_h + 2a_tb_t + 3a_tb_ha_h + \\cdots$\n",
    "Lets denote probabilities where either of them win by $p$, and probabilites where either of them lose by $q$\n",
    "$\\implies \\mathbb{E}(X) = p + 2qp + 3q^2p + \\cdots$ <br/>\n",
    "Solving this geometric series, we get **Expected number of tosses, $\\mathbb{E}(X) = \\frac{1}{p} = 2$**<br/>\n",
    "\n",
    "__(B, extra credit)__<br/>\n",
    "Keeping the same rules of the game, Bob can only win on an even turn, <br/>\n",
    "\n",
    "P(Bob wins) = $a_tb_h$(when he wins on 2nd toss) + $a_tb_ha_tb_t$ (when he wins on 4th toss) + $a_tb_ha_tb_ha_tb_t$ (when he wins on 6th toss) + $\\cdots$ (and so on) <br/>\n",
    "\n",
    "Since it is a fair coin, we can replace those probablities by $\\frac{1}{2}$ and get <br/>\n",
    "\n",
    "P(Bob wins) = $\\frac{1}{4} + \\frac{1}{16} + \\frac{1}{64} + \\cdots$ <br/>\n",
    "\n",
    "Note that the first three terms add up to $\\frac{21}{64}$, which should be precisely Bob's probability of winning.<br/>\n",
    "\n",
    "or, P(Bob wins) =  $\\frac{1}{2^2} + \\frac{1}{2^4} + \\frac{1}{2^6}$, i.e either he wins on 2nd, 4th or 6th toss, so the **game should stop after 6 tosses.**<br/>\n",
    "\n",
    "If Alice starts, the three possible winning moves of Bob should be like this <br/>\n",
    "1. Alice throws T, so Bob gets a turn, and throws T<br/>\n",
    "**Bob wins**<br/>\n",
    "\n",
    "\n",
    "2. Alice throws T, so Bob gets a turn, and throws H<br/>\n",
    "Alice gets a turn, and throws T, so Bob gets a turn, and throws T<br/>\n",
    "**Bob wins**\n",
    "\n",
    "\n",
    "\n",
    "3. Alice throws T, so Bob gets a turn, and throws H<br/>\n",
    "Alice gets a turn, and throws T, so Bob gets a turn, and throws H<br/>\n",
    "Alice gets a turn, and throws T, so Bob gets a turn, and throws T<br/>\n",
    "**Bob wins**\n"
   ]
  },
  {
   "cell_type": "code",
   "execution_count": null,
   "metadata": {},
   "outputs": [],
   "source": []
  },
  {
   "cell_type": "code",
   "execution_count": null,
   "metadata": {},
   "outputs": [],
   "source": []
  }
 ],
 "metadata": {
  "kernelspec": {
   "display_name": "Python 3",
   "language": "python",
   "name": "python3"
  },
  "language_info": {
   "codemirror_mode": {
    "name": "ipython",
    "version": 3
   },
   "file_extension": ".py",
   "mimetype": "text/x-python",
   "name": "python",
   "nbconvert_exporter": "python",
   "pygments_lexer": "ipython3",
   "version": "3.5.5"
  }
 },
 "nbformat": 4,
 "nbformat_minor": 2
}
